Zcash/Circuits/CommitIvk/Composite.lean
@@ -122,11 +122,15 @@ def circuit (wb1 wd1 : WitgenIR Fp 1) :
 
   synthesize := fun (gcfg, lcfg) input => synth wb1 wd1 gcfg lcfg input
 
-  elaborated := fun (gcfg, lcfg) =>
-    { output := fun _ _ => ()
-      regionCount := fun _ => 3
-      output_eq := by intro _ _; rfl
-      regionCount_eq := fun input i => (synth_regionCount wb1 wd1 gcfg lcfg input i).symm }
+  elaborated :=
+    { keygenRequirements :=
+        { gates cfg _ := [gate cfg.1]
+          lookups cfg _ := [LookupRangeCheck.rangeCheckLookup 10 cfg.2] }
+      output _ _ _ := ()
+      regionCount _ := 3
+      output_eq := by intro _ _ _; rfl
+      regionCount_eq := fun (gcfg, lcfg) input i =>
+        (synth_regionCount wb1 wd1 gcfg lcfg input i).symm }
 
   EnvAssumptions := fun (_, lcfg) env =>
     LookupRangeCheck.TableLoaded 10 lcfg env.env ∧
